Work on translations

mechanization/theories/Core/Soundness/Extension/Syntax.v
@@ -7,35 +7,302 @@ Generalizable All Variables.
 
 
 Section Translation.
-  Context (P : PtsSig) (pred_P : PredicativeSig P).
+  Context (P : PtsSig).
+  (* (pred_P : PredicativeSig P). *)
 
   Definition eSig : PtsSig := eP P.
-  Definition ePred : PredicativeSig eSig := epred_P P pred_P.
-  
-  Fixpoint translate_exp (M : exp P) : exp eSig :=
-    match M with
-    | a_st s => @a_st eSig (st_P s)
-    | a_pi r A B => @a_pi eSig _ _ _ (ru_P r) (translate_exp A) (translate_exp B)
-    | a_fn r A M => @a_fn eSig _ _ _ (ru_P r) (translate_exp A) (translate_exp M)
-    | a_app M N => a_app (translate_exp M) (translate_exp N)
-    | a_var n => a_var n
-    | a_sub M σ => a_sub (translate_exp M) (translate_sub σ)
-    end
-      
-  with translate_sub (σ : sub P) : sub eSig :=
-    match σ with
-    | a_id => a_id
-    | a_weaken => a_weaken
-    | a_compose σ τ => a_compose (translate_sub σ) (translate_sub τ)
-    | a_extend σ M => a_extend (translate_sub σ) (translate_exp M)
-    end.
+  (* Definition ePred : PredicativeSig eSig := epred_P P pred_P. *)
 
-  Definition translate_ctx (Γ : ctx P) : ctx eSig := List.map (translate_exp) Γ.
+  Inductive tr_exp : exp P -> exp eSig -> Prop :=
+  | tr_st : forall s, tr_exp {{{ Sort@s }}} (@a_st eSig (st_P s))
+  | tr_pi : forall {s1 s2 s3} (r : Ru P s1 s2 s3) A A' B B',
+      tr_exp A A' -> tr_exp B B' ->
+      tr_exp {{{ Π r A B }}} (@a_pi eSig (st_P s1) (st_P s2) (st_P s3) (ru_P r) A' B')
+  | tr_lam : forall {s1 s2 s3} (r : Ru P s1 s2 s3) A A' M M',
+      tr_exp A A' -> tr_exp M M' ->
+      tr_exp {{{ λ r A M }}} (@a_fn eSig (st_P s1) (st_P s2) (st_P s3) (ru_P r) A' M')
+  | tr_app : forall M M' N N',
+      tr_exp M M' -> tr_exp N N' ->
+      tr_exp {{{ M N }}} {{{ M' N' }}}
+  | tr_var : forall n, tr_exp {{{ #n }}} {{{ #n }}}
+  | tr_clo : forall M M' σ σ',
+      tr_exp M M' -> tr_sub σ σ' ->
+      tr_exp {{{ M[σ] }}} {{{ M'[σ'] }}}
+
+  with tr_sub : sub P -> sub eSig -> Prop :=
+  | tr_id : tr_sub {{{ Id }}} {{{ Id }}}
+  | tr_weaken : tr_sub {{{ Wk }}} {{{ Wk }}}
+  | tr_compose : forall σ σ' τ τ',
+      tr_sub σ σ' -> tr_sub τ τ' ->
+      tr_sub {{{ σ∘τ }}} {{{ σ'∘τ' }}}
+  | tr_extend : forall σ σ' M M',
+      tr_sub σ σ' -> tr_exp M M' ->
+      tr_sub {{{ σ,,M }}} {{{ σ',,M' }}}.
+
+  Inductive tr_ctx : ctx P -> ctx eSig -> Prop :=
+  | tr_nil : tr_ctx {{{ ⋅ }}} {{{ ⋅ }}}
+  | tr_cons : forall Γ Γ' A A',
+      tr_ctx Γ Γ' -> tr_exp A A' ->
+      tr_ctx {{{ Γ, A }}} {{{ Γ', A' }}}.
+
+
+  Scheme tr_exp_mut_ind := Induction for tr_exp Sort Prop
+  with tr_sub_mut_ind := Induction for tr_sub Sort Prop.
+  Combined Scheme tr_mut_ind from
+    tr_exp_mut_ind,
+    tr_sub_mut_ind.
+  
+  #[local]
+  Hint Constructors tr_exp tr_sub tr_ctx : mcpts.
+
+  Lemma tr_functional :
+    (forall M M1, tr_exp M M1 -> forall M2, tr_exp M M2 -> M1 = M2) /\
+      (forall σ σ1, tr_sub σ σ1 -> forall σ2, tr_sub σ σ2 -> σ1 = σ2).
+  Proof using Type.
+    apply tr_mut_ind.
+    1,5,7,8: intros; dependent destruction H; reflexivity.
+    all: intros; dependent destruction H1; (on_all_hyp: fun H => erewrite H in *; eauto).
+  Qed.
+  Lemma tr_functional_ctx : forall Γ Γ1, tr_ctx Γ Γ1 -> forall Γ2, tr_ctx Γ Γ2 -> Γ1 = Γ2.
+  Proof using Type.
+    induction 1; inversion_clear 1; [reflexivity | ].
+    assert (Γ' = Γ'0) by auto.
+    assert (A' = A'0) by (eapply tr_functional; mauto 2).
+    subst.
+    reflexivity.
+  Qed.
+  
+  Corollary tr_exp_functional : forall M M1 M2, tr_exp M M1 -> tr_exp M M2 -> M1 = M2.
+  Proof using Type. intros; eapply tr_functional; eauto. Qed.
+  
+  Corollary tr_sub_functional : forall σ σ1 σ2, tr_sub σ σ1 -> tr_sub σ σ2 -> σ1 = σ2.
+  Proof using Type. intros; eapply tr_functional; eauto. Qed.
+
+  Corollary tr_ctx_functional : forall Γ Γ1 Γ2, tr_ctx Γ Γ1 -> tr_ctx Γ Γ2 -> Γ1 = Γ2.
+  Proof using Type. intros; eapply tr_functional_ctx; eauto. Qed.
+    
+
+  Lemma tr_injective :
+    (forall M1 M, tr_exp M1 M -> forall M2, tr_exp M2 M -> M1 = M2) /\
+      (forall σ1 σ, tr_sub σ1 σ -> forall σ2, tr_sub σ2 σ -> σ1 = σ2).
+  Proof using Type.
+    apply tr_mut_ind.
+    1,5,7,8: intros; dependent destruction H; reflexivity.
+    all: intros; dependent destruction H1; (on_all_hyp: fun H => erewrite H in *; eauto).  
+  Qed.
+  Lemma tr_injective_ctx : forall Γ1 Γ, tr_ctx Γ1 Γ -> forall Γ2, tr_ctx Γ2 Γ -> Γ1 = Γ2.
+  Proof using Type.
+    induction 1; inversion_clear 1; [reflexivity |].
+    assert (Γ = Γ0) by auto.
+    assert (A = A0) by (eapply tr_injective; mauto 2).
+    subst.
+    reflexivity.
+  Qed.    
+
+  Corollary tr_exp_injective : forall M1 M2 M, tr_exp M1 M -> tr_exp M2 M -> M1 = M2.
+  Proof using Type. intros; eapply tr_injective; eauto. Qed.
+  Corollary tr_sub_injective : forall σ1 σ2 σ, tr_sub σ1 σ -> tr_sub σ2 σ -> σ1 = σ2.
+  Proof using Type. intros; eapply tr_injective; eauto. Qed.
+  Corollary tr_ctx_injective : forall Γ1 Γ2 Γ, tr_ctx Γ1 Γ -> tr_ctx Γ2 Γ -> Γ1 = Γ2.
+  Proof using Type. intros; eapply tr_injective_ctx; eauto. Qed.
+    
+  (* Fixpoint translate_exp (M : exp P) : exp eSig := *)
+  (*   match M with *)
+  (*   | a_st s => @a_st eSig (st_P s) *)
+  (*   | a_pi r A B => @a_pi eSig _ _ _ (ru_P r) (translate_exp A) (translate_exp B) *)
+  (*   | a_fn r A M => @a_fn eSig _ _ _ (ru_P r) (translate_exp A) (translate_exp M) *)
+  (*   | a_app M N => a_app (translate_exp M) (translate_exp N) *)
+  (*   | a_var n => a_var n *)
+  (*   | a_sub M σ => a_sub (translate_exp M) (translate_sub σ) *)
+  (*   end *)
+      
+  (* with translate_sub (σ : sub P) : sub eSig := *)
+  (*   match σ with *)
+  (*   | a_id => a_id *)
+  (*   | a_weaken => a_weaken *)
+  (*   | a_compose σ τ => a_compose (translate_sub σ) (translate_sub τ) *)
+  (*   | a_extend σ M => a_extend (translate_sub σ) (translate_exp M) *)
+  (*   end. *)
+
+  (* Definition translate_ctx (Γ : ctx P) : ctx eSig := List.map (translate_exp) Γ. *)
+
+  
 End Translation.
 
-Arguments translate_exp {P}.
-Arguments translate_sub {P}.
-Arguments translate_ctx {P}.
+Arguments tr_exp {P}.
+Arguments tr_st {P}.
+Arguments tr_pi {P} {s1} {s2} {s3}.
+Arguments tr_lam {P} {s1} {s2} {s3}.
+Arguments tr_app {P}.
+Arguments tr_var {P}.
+Arguments tr_clo {P}.
+
+Arguments tr_sub {P}.
+Arguments tr_id {P}.
+Arguments tr_weaken {P}.
+Arguments tr_compose {P}.
+Arguments tr_extend {P}.
+
+Arguments tr_ctx {P}.
+Arguments tr_nil {P}.
+Arguments tr_cons {P}.
+
+
+#[export]
+Hint Resolve tr_exp_functional tr_sub_functional tr_ctx_functional : mcpts.
+
+Ltac functional_tr_rewrite_clear1 :=
+  let tactic_error o1 o2 := fail 3 "tr_functional equality between" o1 "and" o2 "cannot be solved by mauto" in
+  match goal with
+  | H1 : tr_exp ?M ?M1,
+      H2 : tr_exp ?M ?M2 |- _ =>
+      clean replace M2 with M1 by first [solve [mauto 2] | tactic_error M2 M1]; clear H2
+  | H1 : tr_sub ?σ ?σ1,
+      H2 : tr_sub ?σ ?σ2 |- _ =>
+      clean replace σ2 with σ1 by first [solve [mauto 2] | tactic_error σ2 σ1]; clear H2
+  | H1 : tr_ctx ?Γ ?Γ1,
+      H2 : tr_ctx ?Γ ?Γ2 |- _ =>
+      clean replace Γ2 with Γ1 by first [solve [mauto 2] | tactic_error Γ2 Γ1]; clear H2
+  end.
+Ltac functional_tr_rewrite_clear := repeat functional_tr_rewrite_clear1.
+
+#[export]
+Hint Resolve tr_exp_injective tr_sub_injective tr_ctx_injective : mcpts.
+
+Ltac injective_tr_rewrite_clear1 :=
+  let tactic_error o1 o2 := fail 3 "tr_functional equality between" o1 "and" o2 "cannot be solved by mauto" in
+  match goal with
+  | H1 : tr_exp ?M1 ?M,
+      H2 : tr_exp ?M2 ?M |- _ =>
+      clean replace M2 with M1 by first [solve [mauto 2] | tactic_error M2 M1]; clear H2
+  | H1 : tr_sub ?σ1 ?σ,
+      H2 : tr_sub ?σ2 ?σ |- _ =>
+      clean replace σ2 with σ1 by first [solve [mauto 2] | tactic_error σ2 σ1]; clear H2
+  | H1 : tr_ctx ?Γ1 ?Γ,
+      H2 : tr_ctx ?Γ2 ?Γ |- _ =>
+      clean replace Γ2 with Γ1 by first [solve [mauto 2] | tactic_error Γ2 Γ1]; clear H2
+  end.
+Ltac injective_tr_rewrite_clear := repeat injective_tr_rewrite_clear1.
+
+
+Ltac destruct_tr H :=
+  match type of H with
+  | tr_exp {{{ Sort@?s }}} ?M' => dependent destruction H
+  | tr_exp {{{ Π ?r ^?A ^?B }}} ?M' => dependent destruction H
+  | tr_exp {{{ λ ?r ^?A ^?M }}} ?M' => dependent destruction H
+  | tr_exp {{{ ^?M ^?N }}} ?M' => dependent destruction H
+  | tr_exp {{{ #?n }}} ?M' => dependent destruction H
+  | tr_exp {{{ ^?M[^?σ] }}} ?M' => dependent destruction H
+  | tr_sub {{{ Id }}} ?σ' => dependent destruction H
+  | tr_sub {{{ Wk }}} ?σ' => dependent destruction H
+  | tr_sub {{{ ^?σ ∘ ^?τ }}} ?σ' => dependent destruction H
+  | tr_sub {{{ ^?σ,,^?M }}} ?M' => dependent destruction H
+  | tr_ctx {{{ ⋅ }}} ?Γ' => dependent destruction H
+  | tr_ctx {{{ ^?Γ, ^?A }}} ?Γ' => dependent destruction H
+  end;
+  functional_tr_rewrite_clear.
+
+Lemma tr_wf_ctx_lookup {P} : forall {A : typ P} {n Γ A' Γ'},
+    tr_exp A A' ->
+    tr_ctx Γ Γ' ->
+    {{ #n : A ∈ Γ }} ->
+    {{ #n : A' ∈ Γ' }}.
+Proof.
+  intros.
+  gen H H0 A' Γ'.
+  induction H1; simpl;
+    intros * HAA' HΓΓ';
+    inversion_clear HAA'; inversion_clear HΓΓ'.
+  - inversion_clear H2.
+    functional_tr_rewrite_clear.
+    mauto.
+  - inversion_clear H3.
+    econstructor.
+    eapply IHctx_lookup; mauto.
+Qed.
+
+#[export]
+Hint Resolve tr_wf_ctx_lookup : mcpts.
+
+Lemma tr_judg {P} :
+  (forall (Γ : ctx P), {{ ⊢ Γ }} ->
+                  forall Γ',
+                    tr_ctx Γ Γ' ->
+                    {{ ⊢ Γ' }}) /\
+    (forall (Γ : ctx P) Δ, {{ ⊢ Γ ≈ Δ }} ->
+                  forall Γ' Δ',
+                    tr_ctx Γ Γ' -> tr_ctx Δ Δ' ->
+                    {{ ⊢ Γ' ≈ Δ' }}) /\
+    (forall (Γ : ctx P) A M, {{ Γ ⊢ M : A }} ->
+                        forall A' Γ' M',
+                          tr_ctx Γ Γ' -> tr_exp M M' -> tr_exp A A' ->
+                          {{ Γ' ⊢ M' : A' }}) /\
+    (forall (Γ : ctx P) A M N, {{ Γ ⊢ M ≈ N : A }} ->
+                        forall Γ' A' M' N',
+                          tr_ctx Γ Γ' -> tr_exp M M' -> tr_exp N N' -> tr_exp A A' ->
+                          {{ Γ' ⊢ M' ≈ N' : A' }}) /\
+    (forall (Γ : ctx P) A, {{ Γ ⊢ A }} ->
+                      forall Γ' A',
+                        tr_ctx Γ Γ' -> tr_exp A A' ->
+                        {{ Γ' ⊢ A' }}) /\
+    (forall (Γ : ctx P) A B, {{ Γ ⊢ A ≈ B }} ->
+                      forall Γ' A' B',
+                        tr_ctx Γ Γ' -> tr_exp A A' -> tr_exp B B' ->
+                        {{ Γ' ⊢ A' ≈ B' }}) /\
+    (forall (Γ : ctx P) Δ σ, {{ Γ ⊢s σ : Δ }} ->
+                        forall Γ' Δ' σ',
+                          tr_ctx Γ Γ' -> tr_sub σ σ' -> tr_ctx Δ Δ' ->
+                          {{ Γ' ⊢s σ' : Δ' }}) /\
+    (forall (Γ : ctx P) Δ σ τ, {{ Γ ⊢s σ ≈ τ : Δ }} ->
+                        forall Γ' Δ' σ' τ',
+                          tr_ctx Γ Γ' -> tr_sub σ σ' -> tr_sub τ τ' -> tr_ctx Δ Δ' ->
+                          {{ Γ' ⊢s σ' ≈ τ' : Δ' }}).
+Proof.
+  (* apply syntactic_wf_mut_ind. *)
+  (* all: intros; *)
+  (*   (on_all_hyp: destruct_tr); *)
+  (*   econstructor; mauto 2. *)
+
+  (* - eapply H0; mauto 2; *)
+  (*     econstructor; mauto 2. *)
+
+  (* - eapply H0; mauto 2; *)
+  (*     econstructor; mauto 2. *)
+  (* - eapply H1; mauto 2; *)
+  (*     econstructor; mauto 2. *)
+  (* - eapply H2; mauto 2; *)
+  (*     econstructor; mauto 2. *)
+  (* - eapply H3; mauto 2; *)
+  (*     econstructor; mauto 2. *)
+
+  (* - econstructor; mauto 2. *)
+    
+  (* - eapply H; mauto 2;   *)
+  (*     econstructor; mauto 2. *)
+
+  (* - eapply H0; mauto 2; *)
+  (*     econstructor; mauto 2. *)
+
+  (* - eapply H; mauto 2; *)
+  (*     econstructor; mauto 2. *)
+  (* - eapply H0; mauto 2; *)
+  (*     econstructor; mauto 2. *)
+
+  (* - eapply H1; mauto 2; *)
+  (*     econstructor; mauto 2. *)
+
+  (* -  *)
+Admitted.
+
+
+
+
+
+
+    
+(* Arguments translate_exp {P}. *)
+(* Arguments translate_sub {P}. *)
+(* Arguments translate_ctx {P}. *)
 
 Lemma translate_wf_ctx_lookup {P} : forall {A : typ P} {n Γ},
     {{ #n : A ∈ Γ }} ->
@@ -102,4 +369,3 @@ Proof.
   all: try (econstructor; mautosolve 4).
   all: econstructor; [econstructor|]; eauto.
 Qed.
-
